Add profs for program "Smart lighting"

Pattern2_Def.thy
@@ -3,25 +3,27 @@ theory Pattern2_Def
 begin
 
 definition P2all where " P2all s A \<equiv>
-\<forall> s1. consecutive s1 s \<longrightarrow> A s1 s"
+\<forall> s1. consecutive s1 s \<longrightarrow> A s1"
 
 definition P2ex where "P2ex s A \<equiv>
-\<exists> s1. consecutive s1 s \<and> A s1 s"
+\<exists> s1. consecutive s1 s \<and> A s1"
 
 definition P2 where  "P2 s A1 A2 \<equiv> toEnvP s \<and>
 (\<forall> s1 s2. consecutive s1 s2 \<and> substate s2 s \<and> A1 s1 s2 \<longrightarrow> A2 s1 s2)"
 
-lemma P2all_rule: "consecutive s0 s \<Longrightarrow> P2all s A = A s0 s"
-  apply(unfold consecutive_def P2all_def)
+lemma P2all_rule: "consecutive s0 s \<Longrightarrow>  A s0 \<Longrightarrow> P2all s A"
+  apply(unfold  P2all_def)
+  apply simp
   by (metis toEnvNum_eq_imp_eq2)
 
-lemma P2ex_rule: "consecutive s0 s \<Longrightarrow> P2ex s A = A s0 s"
-  apply(unfold consecutive_def P2ex_def)
-  by (metis toEnvNum_eq_imp_eq2)
+lemma P2ex_rule: "consecutive s0 s \<Longrightarrow>  A s0  \<Longrightarrow> P2ex s A"
+  apply(unfold  P2ex_def)
+  by auto
 
 lemma P2_rule: "consecutive s0 s \<Longrightarrow> P2 s0 A1 A2 \<Longrightarrow> (consecutive s0 s \<Longrightarrow> A1 s0 s \<longrightarrow> A2 s0 s) \<Longrightarrow> P2 s A1 A2"
   apply simp
-  apply(unfold P2_def consecutive_def)
+  apply(unfold P2_def)
+  apply simp
   by (metis One_nat_def substate_noteq_imp_substate_of_pred toEnvNum_eq_imp_eq2)
 
 end
