Patterns.thy
@@ -1,0 +1,19 @@
+theory Patterns imports
+Pattern1_Def
+Pattern2_Def
+Pattern3_Def
+Pattern4_Def
+Pattern5_Def
+Pattern6_Def
+Pattern7_Def
+Pattern9_Def
+Pattern10_Def
+Pattern11_Def
+Pattern12_Def
+begin
+
+
+lemma imp_rule: "(A1 \<Longrightarrow> \<not>A1') \<Longrightarrow> (A2 \<Longrightarrow> A2') \<Longrightarrow> A1 \<or> A2 \<Longrightarrow> A1' \<longrightarrow> A2'"
+  by auto
+
+end
