SmartLighting/Proofs_R2.thy
@@ -1,0 +1,108 @@
+theory Proofs_R2
+  imports ExtraInv_R2 Requirements
+begin
+
+definition inv2 where "inv2 s \<equiv> extraInv s \<and> R2 s"
+
+theorem "VC1 inv2 s0"
+  apply(unfold VC1_def inv2_def R2_def P5_1_def P2all_def)
+  using extra1 VC1_def apply auto
+  done
+
+theorem "VC146 inv2 env s0 motion_value light_value"
+  apply(unfold VC146_def inv2_def R2_def)
+  apply(rule impI)
+  apply(rule context_conjI)
+  using extra146 VC146_def apply auto[1]
+  apply(rule conjI)
+   apply simp
+  apply(unfold extraInv_def commonExtraInv_def)
+  apply(erule conjE)+
+  apply(auto simp add:  Pattern5_Def.P5_1_einv2req)
+  done
+
+theorem "VC164 inv2 env s0 motion_value light_value"
+  apply(unfold VC164_def inv2_def R2_def)
+  apply(rule impI)
+  apply(rule context_conjI)
+  using extra164 VC164_def apply auto[1]
+  apply(rule conjI)
+   apply simp
+  apply(unfold extraInv_def commonExtraInv_def)
+  apply(erule conjE)+
+  apply(auto simp add:  Pattern5_Def.P5_1_einv2req)
+  done
+
+theorem "VC182 inv2 env s0 motion_value light_value"
+  apply(unfold VC182_def inv2_def R2_def)
+  apply(rule impI)
+  apply(rule context_conjI)
+  using  VC182_def apply auto[1]
+  apply(rule conjI)
+   apply simp
+  apply(unfold extraInv_def commonExtraInv_def)
+  apply(erule conjE)+
+  apply(auto simp add:  Pattern5_Def.P5_1_einv2req)
+  done
+
+theorem "VC200 inv2 env s0 motion_value light_value"
+  apply(unfold VC200_def inv2_def R2_def)
+  apply(rule impI)
+  apply(rule context_conjI)
+  using extra200 VC200_def apply auto[1]
+  apply(rule conjI)
+   apply simp
+  apply(unfold extraInv_def commonExtraInv_def)
+  apply(erule conjE)+
+  apply(auto simp add:  Pattern5_Def.P5_1_einv2req)
+  done
+
+theorem "VC218 inv2 env s0 motion_value light_value"
+  apply(unfold VC218_def inv2_def R2_def)
+  apply(rule impI)
+  apply(rule context_conjI)
+  using extra218 VC218_def apply auto[1]
+  apply(rule conjI)
+   apply simp
+  apply(unfold extraInv_def commonExtraInv_def)
+  apply(erule conjE)+
+  apply(auto simp add:  Pattern5_Def.P5_1_einv2req)
+  done
+
+theorem "VC236 inv2 env s0 motion_value light_value"
+  apply(unfold VC236_def inv2_def R2_def)
+  apply(rule impI)
+  apply(rule context_conjI)
+  using extra236 VC236_def apply auto[1]
+  apply(rule conjI)
+   apply simp
+  apply(unfold extraInv_def commonExtraInv_def)
+  apply(erule conjE)+
+  apply(auto simp add:  Pattern5_Def.P5_1_einv2req)
+  done
+
+theorem "VC254 inv2 env s0 motion_value light_value"
+  apply(unfold VC254_def inv2_def R2_def)
+  apply(rule impI)
+  apply(rule context_conjI)
+  using extra254 VC254_def apply auto[1]
+  apply(rule conjI)
+   apply simp
+  apply(unfold extraInv_def commonExtraInv_def)
+  apply(erule conjE)+
+  apply(auto simp add:  Pattern5_Def.P5_1_einv2req)
+  done
+
+theorem "VC272 inv2 env s0 motion_value light_value"
+  apply(unfold VC272_def inv2_def R2_def)
+  apply(rule impI)
+  apply(rule context_conjI)
+  using extra272 VC272_def apply auto[1]
+  apply(rule conjI)
+   apply simp
+  apply(unfold extraInv_def commonExtraInv_def)
+  apply(erule conjE)+
+  apply(auto simp add:  Pattern5_Def.P5_1_einv2req)
+  done
+
+end
